

# Differentiation Tutorial Sheet 1

use

— Average rate of change:  $m = \frac{y_2 - y_1}{x_2 - x_1}$

Q1  $y = 3x^2 - 2x$   $x_1 = 1$   $x_2 = 2$

when  $x_1 = 1$   $y_1 = 3(1)^2 - 2(1)$   
 $= 3 - 2$   
 $y_1 = 1$

$(1, 1)$

when  $x_2 = 2$   $y_2 = 3(2)^2 - 2(2)$   
 $= 12 - 4$   
 $y_2 = 8$

$(2, 8)$

$\Rightarrow m = \frac{y_2 - y_1}{x_2 - x_1} = \frac{8 - 1}{2 - 1} = \boxed{7}$  avg. rate of change

Q2  $y = 5x^2 - x$

$x_1 = 0.5$   $y_1 = 5(0.5)^2 - 0.5$   
 $= 0.75$

$(0.5, 0.75)$

$x_2 = 1$   $y_2 = 5(1)^2 - 1$   
 $= 4$

$(1, 4)$

$m = \frac{4 - 0.75}{1 - 0.5} = \frac{3.25}{0.5} = \boxed{6.5}$  avg. rate of change.

$$83. \quad n = 40t - 6t^2$$

$$\begin{aligned} t_1 &= 2 & n_1 &= (40)(2) - 6(2)^2 \\ & & &= 80 - 24 \\ & & n_1 &= 56 \end{aligned}$$

$$\begin{aligned} t_2 &= 4 & n_2 &= 40(4) - 6(4)^2 \\ & & &= 160 - 96 \\ & & n_2 &= 64 \end{aligned}$$

$$M = \frac{64 - 56}{4 - 2} = \frac{8}{2} = \boxed{4} \text{ avg. rate of change.}$$

84 Differentiation using Power Rule  $y = x^n$   
 $\frac{dy}{dx} = nx^{n-1}$

$$\begin{aligned} \text{a. } y &= 3x^5 + 7x^4 + 2x^3 + 11x^2 + 4x + 9 \\ \frac{dy}{dx} &= (3)(5)x^{5-1} + (7)(4)x^{4-1} + (2)(3)x^{3-1} + (11)(2)x^{2-1} + (4)(1)x^{1-1} + 0 \\ &= 15x^4 + 28x^3 + 6x^2 + 22x + 4 \end{aligned}$$

$$\text{b. } s = 5x^2 - 7x + 11$$

$$\begin{aligned} \frac{ds}{dx} &= (5)(2)x^{2-1} - (7)(1)x^{1-1} + 0 \\ &= 10x - 7 \end{aligned}$$

$$\text{c. } r = 3 - 2x - 4x^2 - 10x^3$$

$$\frac{dr}{dx} = -2 - 8x - 30x^2$$



$$d. y = 2\sqrt{x} = 2x^{\frac{1}{2}}$$

$$\begin{aligned} \frac{dy}{dx} &= (2)\left(\frac{1}{2}\right)x^{\frac{1}{2}-1} \\ &= x^{-\frac{1}{2}} = \frac{1}{\sqrt{x}} \end{aligned}$$

Q5  $y = 2x^3 - 3x$  slope of tangent (Derivative) at point  $(2, 10)$  use power Rule.

$$\text{get } \frac{dy}{dx} = 6x^2 - 3$$

$$(2, 10)$$

sub into  $\frac{dy}{dx}$  for  $x \Rightarrow \frac{dy}{dx} = 6(2)^2 - 3$

$$= \boxed{21} \text{ slope of tangent (instantaneous rate of change - the derivative)}$$

Q6.  $y = x^2 + 2x - 3$  at the point  $(-2, -3)$

get slope of tangent:  $\frac{dy}{dx} = 2x + 2$

when  $x = -2$ :  $\frac{dy}{dx} = 2(-2) + 2$

$$= -4 + 2$$

$$\frac{dy}{dx} = -2$$

$2y + 4x - 3 = 0$  use  $y = mx + c$

$$2y = -4x + 3$$

$$y = \frac{-4x}{2} + \frac{3}{2}$$

Parallel

$$y = \boxed{-2x} + 3 \text{ slope } m$$



Q7 i)  $y = 2x^2 - 3x + 6$

$$\frac{dy}{dx} = 4x - 3$$

$$\frac{d^2y}{dx^2} = 4$$

ii)  $y = 4x^4 - 2x^2$

$$\frac{dy}{dx} = 16x^3 - 4x$$

$$\frac{d^2y}{dx^2} = 48x^2 - 4$$

Q8.  $y = \underbrace{(5x+7)}_u \underbrace{(2x+11)}_v$

use Product Rule

$$\frac{df}{dx} = u \frac{dv}{dx} + v \frac{du}{dx}$$

let  $u = 5x + 7$   $\frac{du}{dx} = 5$

$v = 2x + 11$   $\frac{dv}{dx} = 2$

Sub all into the formula.

$$\frac{df}{dx} = (5x+7)(2) + (2x+11)(5)$$

$$= 10x + 14 + 10x + 55$$

$$= 20x + 69$$

Q9  $y = \frac{3x-5}{x^2+1}$   $\begin{matrix} \nearrow u \\ \nwarrow v \end{matrix}$

use Quotient Rule:

$$\frac{df}{dx} = \frac{v \frac{du}{dx} - u \frac{dv}{dx}}{v^2}$$

Let  $u = 3x-5$   $\frac{du}{dx} = 3$

$v = x^2+1$   $\frac{dv}{dx} = 2x$

Sub all into the formula:

$$\frac{df}{dx} = \frac{(x^2+1)(3) - (3x-5)(2x)}{(x^2+1)^2}$$

$$= \frac{3x^2+3 - 6x^2+10x}{(x^2+1)^2}$$

$$\frac{df}{dx} = \frac{-3x^2+10x+3}{(x^2+1)^2}$$